\documentclass{article}
\usepackage{titling}
\usepackage{indentfirst}
\usepackage[export]{adjustbox}
\usepackage{amsmath}
\usepackage{amssymb}

\title{Proofs About Expected Value and Variance}
\author{$\mathbb{L}$umi}
\setlength{\droptitle}{-8em}
\date{\today}

\begin{document}
	
\maketitle

We would like to prove three equations mentioned on Biostatistics course on March the 7th.

\section{Pre-requirements}
Expected values are defined as follows.
\begin{equation}
	E(X) = \sum_x x P_X(x)
\end{equation}

Variances are defined as follows.
\begin{equation}
\begin{aligned}
	\mathrm{Var}(X) &= E([X - E(X)]^2) \\
\end{aligned}
\end{equation}

\section{Random Variables Built on Random Variables}

Suppose we have random variables $X$ and $Y$. $Y$ and $X$ are related through the funciton $y = f(x)$. We would like to prove that

\begin{equation}
	E(Y) = \sum_x g(x)P_X(x)
\end{equation}

We start from the basic definition of expected values.

\begin{equation}
\begin{aligned}
	E(Y) &= \sum_y y P_Y(y) \\
	&= \sum_x g(x) P_{g(X)}(g(x))
\end{aligned}
\end{equation}

Thus, what we need to prove is $P_{g(X)}(g(x)) = P_X(x)$.

\begin{equation}
\begin{aligned}
	P_{g(x)} (g(x)) &= \sum P(g(X) = g(x)) \\
	&= \sum P(X = g^{-1}[g(x)]) \\
	&= \sum P(X=x) \\
	&= P_X(x)
\end{aligned}	
\end{equation}

\section{Nudging $X$ in a Linear Way}
The second equation to prove is when we nudge $X$ a bit and see what happens to the expected value of $X$.

\begin{equation}
	E(\alpha X+\beta) = \alpha E(X) + \beta
\end{equation}

This is quite easy to prove with the basic definition.

\begin{equation}
	\begin{aligned}
		E(\alpha X + \beta) &= \sum_x (\alpha x + \beta)P(\alpha x + \beta) \\
		&=\sum_x \alpha x P(\alpha x + \beta) + \sum_x \beta P(\alpha x + \beta) \\
	\end{aligned}
\end{equation} 

We know that,
\begin{equation}
			\sum_{x} P(\alpha x + \beta) = 1, P(\alpha x + \beta) = P(x)
\end{equation}

So
\begin{equation}
\begin{aligned}
		E(\alpha x + \beta) &= \alpha \sum_x x P(x) + \beta \\
		&= \alpha E(X) + \beta
\end{aligned}
\end{equation}

	
\end{document}














































